main/hl/solutions/lean/HL/Hoare.lean
@@ -3450,4 +3450,4 @@ theorem assert_assume_example :
 
 end HoareAssertAssume
 
--- Source revision: 1a547d1, committed 2026-09-18 21:25 UTC
+-- Source revision: cdbd63d, committed 2026-09-21 21:19 UTC
