main/hl/student/lean/HL.lean
@@ -5,4 +5,4 @@ import HL.Equiv
 import HL.Hoare
 import HL.Hoare2
 
--- Source revision: 1a547d1, committed 2026-09-18 21:25 UTC
+-- Source revision: cdbd63d, committed 2026-09-21 21:19 UTC
