main/hl/terse/lean/HL/Hoare.lean
@@ -1478,4 +1478,4 @@ theorem hoare_while {P : Assertion} {b : Bexp} {c : Com}
 --  the rules of Hoare logic as a closed world for reasoning
 --  about programs.
 
--- Source revision: 1a547d1, committed 2026-09-18 21:25 UTC
+-- Source revision: cdbd63d, committed 2026-09-21 21:19 UTC
