main/lf/solutions/lean/LF/Lists.lean
@@ -1347,4 +1347,4 @@ end PartialMap
 
 end Lists
 
--- Source revision: 1a547d1, committed 2026-09-18 21:25 UTC
+-- Source revision: cdbd63d, committed 2026-09-21 21:19 UTC
