main/lf/solutions/lean/LF/UsingLean.lean
@@ -526,4 +526,4 @@ theorem Nat.double_mul (n : Nat) : n.double = 2 * n := by
 --  With these tools in hand, we can begin to prove properties about more
 --  sophisticated forms of data, beginning with `Lists`.
 
--- Source revision: 1a547d1, committed 2026-09-18 21:25 UTC
+-- Source revision: cdbd63d, committed 2026-09-21 21:19 UTC
