main/ts/solutions/lean/TS/Preface.lean
@@ -72,4 +72,4 @@ import SFLCompat
 --  Note to developers (Benjamin Pierce @bcpierce00):
 --      Other funding should be acknowledged here...
 
--- Source revision: 1a547d1, committed 2026-09-18 21:25 UTC
+-- Source revision: cdbd63d, committed 2026-09-21 21:19 UTC
