main/ts/solutions/lean/TS/Sub.lean
@@ -2385,4 +2385,4 @@ end FormalThoughtExercises
 
 end StlcSub
 
--- Source revision: 1a547d1, committed 2026-09-18 21:25 UTC
+-- Source revision: cdbd63d, committed 2026-09-21 21:19 UTC
