main/ts/student/lean/TS/MoreStlc.lean
@@ -2160,4 +2160,4 @@ theorem preservation (t t' : Tm) (τ : Ty)
 
 end StlcExtended
 
--- Source revision: 1a547d1, committed 2026-09-18 21:25 UTC
+-- Source revision: cdbd63d, committed 2026-09-21 21:19 UTC
