main/ts/terse/lean/TS/MoreStlc.lean
@@ -1018,4 +1018,4 @@ attribute [ExtStlcEval] Tm.IsValue.abs Tm.IsValue.nat Tm.IsValue.sumInl Tm.IsVal
 
 end StlcExtended
 
--- Source revision: 1a547d1, committed 2026-09-18 21:25 UTC
+-- Source revision: cdbd63d, committed 2026-09-21 21:19 UTC
