main/ts/terse/lean/TS/Smallstep.lean
@@ -1049,4 +1049,4 @@ macro_rules
 example : (.p (.c 3) (.p (.c 3) (.c 4))) ⟶* (.c 10) := by
   normalize using SimpleArith
 
--- Source revision: 1a547d1, committed 2026-09-18 21:25 UTC
+-- Source revision: cdbd63d, committed 2026-09-21 21:19 UTC
