main/ts/terse/lean/TS/Sub.lean
@@ -1255,4 +1255,4 @@ theorem preservation {t t' : Tm} {τ : Ty}
 
 end StlcSub
 
--- Source revision: 1a547d1, committed 2026-09-18 21:25 UTC
+-- Source revision: cdbd63d, committed 2026-09-21 21:19 UTC
